bridge ready body callbacks

rocq/theories/TypeSystem/TypeSafetyDirectCallRoute.v
@@ -909,6 +909,87 @@ Definition eval_preserves_typing_roots_store_safe_synthetic_direct_call_ready_bo
   eval_preserves_typing_roots_store_safe_synthetic_direct_call_ready_body_call_store_safe_callback_height_statement_in_env_family
     (global_env_local_bounds_family base).
 
+Definition eval_preserves_typing_roots_store_safe_ready_body_call_store_safe_callback_height_statement_at
+    (env : global_env) (fdef : fn_def) : Prop :=
+  forall fname fcall used used' s_args s_body vs ret R_args
+      arg_roots fname_body args_body T_body Gamma_out R_body roots_body,
+    In fdef (env_fns env) ->
+    fn_name fdef = fname ->
+    alpha_rename_fn_def used fdef = (fcall, used') ->
+    direct_call_target_expr (fn_body fcall) =
+      Some (fname_body, args_body, ECall fname_body args_body) ->
+    store_safe_function_value_call_args
+      (global_env_with_local_bounds env (fn_bounds fcall)) args_body ->
+    preservation_ready_args args_body ->
+    typed_env_roots (global_env_with_local_bounds env (fn_bounds fcall))
+      (fn_outlives fcall) (fn_lifetimes fcall)
+      (call_param_root_env (fn_params fcall) arg_roots R_args)
+      (sctx_of_ctx (params_ctx (fn_params fcall)))
+      (ECall fname_body args_body) T_body (sctx_of_ctx Gamma_out) R_body
+      roots_body ->
+    fn_env_unique_by_name (global_env_with_local_bounds env (fn_bounds fcall)) ->
+    fn_root_shadow_ready_body_summary_evidence_at
+      (global_env_with_local_bounds env (fn_bounds fcall)) fname_body ->
+    direct_call_callee_body_root_ready_body_evidence_at
+      (global_env_with_local_bounds env (fn_bounds fcall)) fname_body ->
+    store_typed_prefix (global_env_with_local_bounds env (fn_bounds fcall))
+      (bind_params (fn_params fcall) vs s_args)
+      (sctx_of_ctx (params_ctx (fn_params fcall))) ->
+    store_roots_within
+      (call_param_root_env (fn_params fcall) arg_roots R_args)
+      (bind_params (fn_params fcall) vs s_args) ->
+    store_no_shadow (bind_params (fn_params fcall) vs s_args) ->
+    root_env_no_shadow
+      (call_param_root_env (fn_params fcall) arg_roots R_args) ->
+    root_env_store_roots_named
+      (call_param_root_env (fn_params fcall) arg_roots R_args)
+      (bind_params (fn_params fcall) vs s_args) ->
+    root_env_store_keys_named
+      (call_param_root_env (fn_params fcall) arg_roots R_args)
+      (bind_params (fn_params fcall) vs s_args) ->
+    eval (global_env_with_local_bounds env (fn_bounds fcall))
+      (bind_params (fn_params fcall) vs s_args)
+      (ECall fname_body args_body) s_body ret ->
+    forall n_body_call,
+    direct_call_eval_height
+      (global_env_with_local_bounds env (fn_bounds fcall))
+      (bind_params (fn_params fcall) vs s_args)
+      (ECall fname_body args_body) s_body ret n_body_call ->
+    store_typed_prefix (global_env_with_local_bounds env (fn_bounds fcall))
+      s_body (sctx_of_ctx Gamma_out) /\
+    value_has_type (global_env_with_local_bounds env (fn_bounds fcall))
+      s_body ret T_body /\
+    store_ref_targets_preserved
+      (global_env_with_local_bounds env (fn_bounds fcall))
+      (bind_params (fn_params fcall) vs s_args) s_body /\
+    store_roots_within R_body s_body /\
+    value_roots_within roots_body ret /\
+    store_no_shadow s_body /\
+    root_env_no_shadow R_body.
+
+Lemma eval_preserves_typing_roots_store_safe_synthetic_direct_call_ready_body_call_store_safe_callback_height_statement_at_of_ready_body_at :
+  forall env fdef,
+    eval_preserves_typing_roots_store_safe_ready_body_call_store_safe_callback_height_statement_at
+      env fdef ->
+    eval_preserves_typing_roots_store_safe_synthetic_direct_call_ready_body_call_store_safe_callback_height_statement_at
+      env fdef.
+Proof.
+  intros env fdef Hready.
+  unfold
+    eval_preserves_typing_roots_store_safe_ready_body_call_store_safe_callback_height_statement_at,
+    eval_preserves_typing_roots_store_safe_synthetic_direct_call_ready_body_call_store_safe_callback_height_statement_at
+    in *.
+  intros fname fcall used used' s_args s_body vs ret R_args
+    arg_roots fname_body args_body T_body Gamma_out R_body roots_body
+    Hin Hname Hrename Htarget Hsafe Hready_args Htyped Hunique
+    Hsummary Hevidence Hstore Hroots Hshadow Hrn Hnamed Hkeys Heval
+    n_body_call Hheight.
+  eapply Hready; try eassumption.
+  - intros fcallee Hlookup. left. exact (Hsummary fcallee Hlookup).
+  - eapply direct_call_callee_body_root_ready_body_evidence_at_of_synthetic.
+    exact Hevidence.
+Qed.
+
 
 Theorem eval_preserves_typing_roots_store_safe_synthetic_direct_call_ready_body_call_store_safe_callback_height_statement_in_env_family_of_summary_at_prefix_call_statement_evidence_at_height :
   forall env_family,
